Adding more functions to export_code

formalization/mfotl/code/Monitor_Code.thy
@@ -996,6 +996,12 @@ definition specialized_set :: "(MFOTL.name \<times> event_data list) list \<Righ
 definition ed_set :: "event_data list \<Rightarrow> event_data set" where
   "ed_set = set"
 
+definition sum_nat :: "nat \<Rightarrow> nat \<Rightarrow> nat" where
+  "sum_nat m n = m + n"
+
+definition sub_nat :: "nat \<Rightarrow> nat \<Rightarrow> nat" where
+  "sub_nat m n = m - n"
+
 lift_definition abs_part :: "(event_data set \<times> 'a) list \<Rightarrow> (event_data, 'a) part" is
   "\<lambda>xs.
    let Ds = map fst xs in
@@ -1011,7 +1017,7 @@ lemma check_all_check_one: "check_all \<sigma> \<phi> e = (distinct_paths e \<an
     (auto simp: compatible_vals_def)
 
 export_code interval enat nat_of_integer integer_of_nat
-  STT MFOTL.TT Inl EInt MFOTL.Var Leaf set
+  STT MFOTL.TT Inl EInt MFOTL.Var Leaf set part_hd sum_nat sub_nat
   check_all_specialized trace_of_list_specialized specialized_set ed_set abs_part
   in OCaml module_name MFOTL_Explanator2 file_prefix "MFOTL_checker"
 
